verified mov instruction with "register" destination addressing mode

src/verification/Contracts.v
@@ -266,13 +266,14 @@ Module Import MSP430Specification <: Specification MSP430Base MSP430Signature MS
           asn_accessible_addresses "pc" "ipectl" "segb1" "segb2";
       |}.
 
+    (*
     Definition lemma_change_accessible_pc : SepLemma change_accessible_pc :=
       {| lemma_logic_variables :=
           [ "ipectl" :: ty.wordBits; "segb1" :: ty.wordBits; "segb2" :: ty.wordBits
-          ; "pc_old2" :: ty.wordBits; "pc_new" :: ty.wordBits
+          ; "pc_old" :: ty.wordBits; "pc_new" :: ty.wordBits
           ];
 
-        lemma_patterns := [term_var "pc_old2"];
+        lemma_patterns := [term_var "pc_old"];
 
         lemma_precondition :=
             PC_reg         ↦ term_var "pc_new"
@@ -297,6 +298,7 @@ Module Import MSP430Specification <: Specification MSP430Base MSP430Signature MS
 
           ∗ asn_accessible_addresses "pc_new" "ipectl" "segb1" "segb2";
       |}.
+     *)
 
     (* Foreign function contracts *)
 
@@ -492,9 +494,7 @@ Module Import MSP430Specification <: Specification MSP430Base MSP430Signature MS
 
           ∗ asn_untrusted
               (term_var "ipectl") (term_var "segb1")
-              (term_var "segb2") (term_var "pc_old")
-
-          ∗ asn_accessible_addresses "pc_old" "ipectl" "segb1" "segb2";
+              (term_var "segb2") (term_var "pc_old");
 
         sep_contract_result          := "u";
         sep_contract_postcondition   :=
@@ -512,9 +512,7 @@ Module Import MSP430Specification <: Specification MSP430Base MSP430Signature MS
           (*   (* TODO useful? *)
           (*   ∗ asn_access_allowed *)
           (*       (term_var "ipectl") (term_var "segb1") (term_var "segb2") *)
-          (*       (term_enum Eaccess_mode X) (term_var "pc_old") (term_var "pc_new")) *) *)
-
-            ∗ asn_accessible_addresses "pc_new" "ipectl" "segb1" "segb2");
+          (*       (term_enum Eaccess_mode X) (term_var "pc_old") (term_var "pc_new")) *) *));
       |}.
 
     Definition sep_contract_fetch :
@@ -523,13 +521,13 @@ Module Import MSP430Specification <: Specification MSP430Base MSP430Signature MS
       sep_contract_logic_variables :=
         [ "mpuctl0" :: ty.wordBits; "ipectl" :: ty.wordBits
         ; "segb1" :: ty.wordBits; "segb2" :: ty.wordBits
-        ; "pc" :: ty.wordBits; "pc_new" :: ty.wordBits
+        ; "pc_old" :: ty.wordBits; "pc_new" :: ty.wordBits
         ; "u" :: ty.unit ];
 
       sep_contract_localstore := [ term_var "u" ];
 
       sep_contract_precondition :=
-          PC_reg         ↦ term_var "pc"
+          PC_reg         ↦ term_var "pc_old"
         ∗ MPUCTL0_reg    ↦ term_var "mpuctl0"
         ∗ MPUIPC0_reg    ↦ term_var "ipectl"
         ∗ MPUIPSEGB1_reg ↦ term_var "segb1"
@@ -537,9 +535,9 @@ Module Import MSP430Specification <: Specification MSP430Base MSP430Signature MS
 
         ∗ asn_untrusted
             (term_var "ipectl") (term_var "segb1")
-            (term_var "segb2") (term_var "pc")
+            (term_var "segb2") (term_var "pc_old")
 
-        ∗ asn_accessible_addresses "pc" "ipectl" "segb1" "segb2";
+        ∗ asn_accessible_addresses "pc_old" "ipectl" "segb1" "segb2";
 
       sep_contract_result          := "v";
       sep_contract_postcondition   :=
@@ -548,23 +546,19 @@ Module Import MSP430Specification <: Specification MSP430Base MSP430Signature MS
         ∗ MPUIPSEGB1_reg ↦ term_var "segb1"
         ∗ MPUIPSEGB2_reg ↦ term_var "segb2"
 
+        ∗ asn_accessible_addresses "pc_old" "ipectl" "segb1" "segb2"
+
         ∗ ∃ "pc_new",
-          ( term_var "pc_new" = term_word_plus 2 (term_unsigned (term_var "pc"))
+          ( term_var "pc_new" = term_word_plus 2 (term_unsigned (term_var "pc_old"))
 
           ∗ PC_reg ↦ term_var "pc_new"
 
+          (* TODO useful? *)
           (* ∗ asn_access_allowed *)
           (*     (term_var "ipectl") (term_var "segb1") (term_var "segb2") *)
           (*     (term_enum Eaccess_mode X) (term_var "pc") (term_var "pc_new") *)
 
-          (* questo è nell'heap ma aggiungendolo viene fuori False... *)
-          ∗ (asn.chunk (chunk_user accessible_addresses
-              [ (term_word_plus 2 (term_unsigned (term_var "pc")))
-              ; term_var "ipectl"
-              ; term_var "segb1"
-              ; term_var "segb2" ]))
-          (* ∗ asn_accessible_addresses "pc_new" "ipectl" "segb1" "segb2" *)
-);
+          );
     |}.
 
     Definition sep_contract_read_indexed : SepContractFun read_indexed :=
@@ -572,8 +566,8 @@ Module Import MSP430Specification <: Specification MSP430Base MSP430Signature MS
         sep_contract_logic_variables :=
           [ "mpuctl0" :: ty.wordBits; "ipectl" :: ty.wordBits
           ; "segb1" :: ty.wordBits; "segb2" :: ty.wordBits
-          ; "pc" :: ty.wordBits
-          ; "bw" :: ty.enum Ebw; "reg" :: ty.enum Eregister; "am" :: ty.enum Eam
+          ; "pc_old" :: ty.wordBits; "pc_new" :: ty.wordBits
+          ; "bw" :: ty.enum Ebw; "reg" :: ty.enum Eregister
           ];
 
         sep_contract_localstore := [term_var "bw"; term_var "reg"];
@@ -581,32 +575,78 @@ Module Import MSP430Specification <: Specification MSP430Base MSP430Signature MS
         sep_contract_precondition :=
             asn_exist_registers
 
-          ∗ PC_reg         ↦ term_var "pc"
+          ∗ PC_reg         ↦ term_var "pc_old"
           ∗ MPUCTL0_reg    ↦ term_var "mpuctl0"
           ∗ MPUIPC0_reg    ↦ term_var "ipectl"
           ∗ MPUIPSEGB1_reg ↦ term_var "segb1"
           ∗ MPUIPSEGB2_reg ↦ term_var "segb2"
 
-          ∗ asn_accessible_addresses "pc" "ipectl" "segb1" "segb2"
+          ∗ asn_accessible_addresses "pc_old" "ipectl" "segb1" "segb2"
 
           ∗ asn_untrusted
               (term_var "ipectl") (term_var "segb1")
-              (term_var "segb2") (term_var "pc")
-
-          ∗ term_var "bw" = term_enum Ebw BYTE_INSTRUCTION
-          ∗ term_var "reg" = term_enum Eregister SRCG1 (* XXX R4 *)
-          ∗ term_var "am" = term_enum Eam INDEXED_MODE;
+              (term_var "segb2") (term_var "pc_old");
 
         sep_contract_result          := "v";
-        sep_contract_postcondition   := ⊤
-          (*   asn_exist_registers *)
-          (* ∗ PC_reg         ↦ term_word_plus 2 (term_unsigned (term_var "pc")) *)
-          (* ∗ MPUCTL0_reg    ↦ term_var "mpuctl0" *)
-          (* ∗ MPUIPC0_reg    ↦ term_var "ipectl" *)
-          (* ∗ MPUIPSEGB1_reg ↦ term_var "segb1" *)
-          (* ∗ MPUIPSEGB2_reg ↦ term_var "segb2" *)
-          (* ∗ asn_accessible_addresses "pc" "ipectl" "segb1" "segb2" *); (* XXX pc +2 *)
+        sep_contract_postcondition   :=
+            asn_exist_registers
+
+            (* pc_old + 2 except when reading from CG2 *)
+          ∗ (∃ "pc_new", PC_reg ↦ term_var "pc_new")
+
+          ∗ MPUCTL0_reg    ↦ term_var "mpuctl0"
+          ∗ MPUIPC0_reg    ↦ term_var "ipectl"
+          ∗ MPUIPSEGB1_reg ↦ term_var "segb1"
+          ∗ MPUIPSEGB2_reg ↦ term_var "segb2"
+
+          ∗ asn_accessible_addresses "pc_old" "ipectl" "segb1" "segb2";
       |}.
+
+    Definition sep_contract_read_indirect : SepContractFun read_indirect :=
+      {|
+        sep_contract_logic_variables :=
+          [ "mpuctl0" :: ty.wordBits; "ipectl" :: ty.wordBits
+          ; "segb1" :: ty.wordBits; "segb2" :: ty.wordBits
+          ; "pc_old" :: ty.wordBits; "pc_new" :: ty.wordBits
+          ; "bw" :: ty.enum Ebw; "reg" :: ty.enum Eregister
+          ];
+
+        sep_contract_localstore := [term_var "bw"; term_var "reg"];
+
+        sep_contract_precondition :=
+            asn_exist_registers
+
+          ∗ PC_reg         ↦ term_var "pc_old"
+          ∗ MPUCTL0_reg    ↦ term_var "mpuctl0"
+          ∗ MPUIPC0_reg    ↦ term_var "ipectl"
+          ∗ MPUIPSEGB1_reg ↦ term_var "segb1"
+          ∗ MPUIPSEGB2_reg ↦ term_var "segb2"
+
+          ∗ asn_accessible_addresses "pc_old" "ipectl" "segb1" "segb2"
+
+          ∗ asn_untrusted
+              (term_var "ipectl") (term_var "segb1")
+              (term_var "segb2") (term_var "pc_old");
+
+        sep_contract_result          := "v";
+        sep_contract_postcondition   :=
+            asn_exist_registers
+
+          (* always pc_old, but the implementation calls read
+             so would have to make read_indexed's contract more
+             precise to prove that pc_new = pc_old *)
+          ∗ (∃ "pc_new", PC_reg ↦ term_var "pc_new")
+
+          ∗ MPUCTL0_reg    ↦ term_var "mpuctl0"
+          ∗ MPUIPC0_reg    ↦ term_var "ipectl"
+          ∗ MPUIPSEGB1_reg ↦ term_var "segb1"
+          ∗ MPUIPSEGB2_reg ↦ term_var "segb2"
+
+          ∗ asn_accessible_addresses "pc_old" "ipectl" "segb1" "segb2";
+      |}.
+
+    Definition sep_contract_read_autoincrement : SepContractFun read_autoincrement
+      := sep_contract_read_indirect.
 
     Definition sep_contract_read_mpu_reg_byte : SepContractFun read_mpu_reg_byte :=
       {|
@@ -617,14 +657,15 @@ Module Import MSP430Specification <: Specification MSP430Base MSP430Signature MS
         sep_contract_postcondition := asn_exist_mpu_registers;
       |}.
 
-
     Definition sep_contract_execute_move : SepContractFun execute :=
       {|
         sep_contract_logic_variables :=
           [ "mpuctl0" :: ty.wordBits; "ipectl" :: ty.wordBits
           ; "segb1" :: ty.wordBits; "segb2" :: ty.wordBits
-          ; "pc" :: ty.wordBits
-          ; "instr" :: ty.union Uast
+          ; "pc_old" :: ty.wordBits; "pc_new" :: ty.wordBits
+          ; "instr" :: ty.union Uast; "bw" :: ty.enum Ebw
+          ; "src_reg" :: ty.enum Eregister; "dest_reg" :: ty.enum Eregister
+          ; "src_am" :: ty.enum Eam
           ];
 
         sep_contract_localstore := [term_var "instr"];
@@ -632,35 +673,43 @@ Module Import MSP430Specification <: Specification MSP430Base MSP430Signature MS
         sep_contract_precondition :=
             asn_exist_registers
 
-          ∗ PC_reg         ↦ term_var "pc"
+          ∗ PC_reg         ↦ term_var "pc_old"
           ∗ MPUCTL0_reg    ↦ term_var "mpuctl0"
           ∗ MPUIPC0_reg    ↦ term_var "ipectl"
           ∗ MPUIPSEGB1_reg ↦ term_var "segb1"
           ∗ MPUIPSEGB2_reg ↦ term_var "segb2"
 
-          ∗ asn_accessible_addresses "pc" "ipectl" "segb1" "segb2"
+          ∗ asn_accessible_addresses "pc_old" "ipectl" "segb1" "segb2"
 
           ∗ asn_untrusted
               (term_var "ipectl") (term_var "segb1")
-              (term_var "segb2") (term_var "pc")
+              (term_var "segb2") (term_var "pc_old")
 
           ∗ term_var "instr" =
               term_union Uast Kdoubleop
-                (term_val (unionk_ty Uast Kdoubleop)
-                   (tt, MOV, BYTE_INSTRUCTION, R4, INDEXED_MODE, R5, REGISTER_MODE));
+                (term_tuple
+                   [term_val (ty.enum Edoubleop) MOV;
+                    term_var "bw";
+                    term_var "src_reg";
+                    term_var "src_am";
+                    (* term_val (ty.enum Eam) INDEXED_MODE; *)
+                    term_var "dest_reg";
+                    term_val (ty.enum Eam) REGISTER_MODE]);
 
         sep_contract_result          := "u";
         sep_contract_postcondition   :=
             term_var "u" = term_val ty.unit tt
+
           ∗ asn_exist_registers
 
-          ∗ PC_reg         ↦ term_var "pc"
           ∗ MPUCTL0_reg    ↦ term_var "mpuctl0"
           ∗ MPUIPC0_reg    ↦ term_var "ipectl"
           ∗ MPUIPSEGB1_reg ↦ term_var "segb1"
           ∗ MPUIPSEGB2_reg ↦ term_var "segb2"
 
-          ∗ asn_accessible_addresses "pc" "ipectl" "segb1" "segb2";
+          ∗ (∃ "pc_new", PC_reg ↦ term_var "pc_new")
+
+          ∗ asn_accessible_addresses "pc_old" "ipectl" "segb1" "segb2";
       |}.
 
     Definition sep_contract_execute_jump :
@@ -777,6 +826,10 @@ Module Import MSP430Specification <: Specification MSP430Base MSP430Signature MS
         | check_byte_access => Some sep_contract_check_byte_access
         | setPC => Some sep_contract_set_pc
         | incPC => Some sep_contract_inc_pc
+        | fetch => Some sep_contract_fetch
+        | read_indexed => Some sep_contract_read_indexed
+        | read_indirect => Some sep_contract_read_indirect
+        | read_autoincrement => Some sep_contract_read_autoincrement
 
           (* | execute => Some sep_contract_execute *)
         | _ => None
@@ -797,7 +850,7 @@ Module Import MSP430Specification <: Specification MSP430Base MSP430Signature MS
         match l with
         | extract_accessible_ptsto => lemma_extract_accessible_ptsto
         | return_accessible_ptsto => lemma_return_accessible_ptsto
-        | change_accessible_pc => lemma_change_accessible_pc
+        (* | change_accessible_pc => lemma_change_accessible_pc *)
         end.
   End ContractDefKit.
 End MSP430Specification.
@@ -831,111 +884,18 @@ Ltac symbolic_simpl_erasure :=
   compute;
   constructor;
   cbn.
-(*
-Lemma valid_contract_fetch : Symbolic.ValidContract sep_contract_fetch fun_fetch.
-Proof.
-  compute.
-  constructor.
-  cbn [SymProp.safe instprop instprop_formula].
-  intros.
-
-  exists [bv 0]. exists [bv 0]. exists [bv 0]. exists [bv 0]. intro.
-  split.
-
-  
-  intros until v5.
-  intros Henabled Huntrusted _.
-  exists v0.
-  exists v1.
-  exists v2.
-  exists v3.                (* v4? *)
-  intro.
-  repeat split.
-  - intros H_pc_untrusted_left.
-    exists [bv 0].
-    repeat split.
-    + assumption.
-    + assumption.
-    + 
-      left.
-      cbn.
-      cbn in H_pc_untrusted_left.
-      replace (bv.unsigned v3) with (bv.unsigned v3 + 0) by ring.
-      rewrite Z.add_comm with (n := 8).
-      apply Z.add_lt_mono; [assumption | reflexivity].
-    +  intros ? H_pc_plus_2_unprotected ?.
-
-
-
-  intros until v6.
-  intros _ Huntrusted _.
-  repeat split.
-  - intros H_pc_untrusted_left.
-    exists [bv 0].
-    repeat split.
-    + left.
-      cbn.
-      cbn in H_pc_untrusted_left.
-      replace (bv.unsigned v3) with (bv.unsigned v3 + 0) by ring.
-      rewrite Z.add_comm with (n := 8).
-      apply Z.add_lt_mono; [assumption | reflexivity].
-    +  intros ? H_pc_plus_2_unprotected ?.
-
-Lemma valid_contract_read_indexed : Symbolic.ValidContractWithFuel 100 sep_contract_read_indexed fun_read_indexed.
-Proof.
-  compute.
-  constructor.
-  cbn [SymProp.safe instprop instprop_formula].
-  intros until v20.
-  intros _ Huntrusted _.
-
-  repeat split.
-  - intros H_pc_untrusted_left.
-    exists [bv 0].
-    repeat split.
-    + left.
-      cbn.
-      cbn in H_pc_untrusted_left.
-      replace (bv.unsigned v3) with (bv.unsigned v3 + 0) by ring.
-      rewrite Z.add_comm with (n := 8).
-      apply Z.add_lt_mono; [assumption | reflexivity].
-    +  intros ? H_pc_plus_2_unprotected ?.
-
-
-
-    intros ? H_pc_plus_2_unprotected ?.
-
--
-
-
-
-
-  exists [bv [16] 4242].
-  exists [bv [16] 3131].
-  exists [bv [16] 9797].
-  exists [bv [16] 5656].
-  intros.
-  repeat split;
-    try exact [bv 0];
-    intros ? H_pc_plus_2_unprotected H;
-    exists [bv [16] 1111];
-    exists [bv [16] 2222];
-    exists [bv [16] 3333];
-    exists [bv [16] 4444];
-    intros;
-    cbn;
-    (split; [|reflexivity]);
-    unfold bv.add;
-    cbn;
-    rewrite <-bv.of_Z_add, <-bv.of_N_add, bv.of_Z_unsigned, bv.of_N_bin, bv.add_comm;
-    reflexivity.
-Qed.
 
 Lemma valid_contract_execute_move : Symbolic.ValidContractWithFuel 100 sep_contract_execute_move fun_execute.
 Proof.
   compute.
+  constructor.
+  cbn [SymProp.safe instprop instprop_formula].
+  repeat split; intros; exists [bv 0]; split; [assumption|exact I].
+Qed.
 
-  *)
+
+
+
 
 
 Lemma valid_contract_check_byte_access : Symbolic.ValidContractReflect sep_contract_check_byte_access fun_check_byte_access.
@@ -949,13 +909,57 @@ Proof. symbolic_simpl_reflect. Qed.
 
 Lemma valid_contract_execute_inc_pc : Symbolic.ValidContract sep_contract_inc_pc fun_incPC.
 Proof.
+  compute. constructor. cbn [SymProp.safe instprop instprop_formula].
+  intros.
+  repeat split;
+    cbn;
+    rewrite <-bv.of_Z_add, bv.of_Z_unsigned, bv.add_comm;
+    reflexivity.
+Qed.
+
+Lemma valid_contract_fetch : Symbolic.ValidContract sep_contract_fetch fun_fetch.
+Proof.
   compute.
   constructor.
   cbn [SymProp.safe instprop instprop_formula].
 
-  intros. split. split. intros.
+  intros.
+  exists v0. exists v1. exists v2. exists v3.
+  intro.
+  repeat split;
+    intros;
+    exists v; exists v4;
+    repeat split; assumption.
+Qed.
 
-  symbolic_simpl_reflect. Qed.
+Lemma valid_contract_read_indexed : Symbolic.ValidContractWithFuel 100 sep_contract_read_indexed fun_read_indexed.
+Proof.
+  compute.
+  constructor.
+  cbn [SymProp.safe instprop instprop_formula].
+
+  intros.
+  repeat split; intros; exists [bv 0];
+    (split; [assumption | intros; repeat exists [bv 0]; exact I]).
+Qed.
+
+Lemma valid_contract_read_indirect : Symbolic.ValidContractWithFuel 100 sep_contract_read_indirect fun_read_indirect.
+Proof.
+  compute.
+  constructor.
+  cbn [SymProp.safe instprop instprop_formula].
+
+  intros. repeat split; assumption.
+Qed.
+
+Lemma valid_contract_read_autoincrement : Symbolic.ValidContractWithFuel 100 sep_contract_read_autoincrement fun_read_autoincrement.
+Proof.
+  compute.
+  constructor.
+  cbn [SymProp.safe instprop instprop_formula].
+
+  intros. repeat split; assumption.
+Qed.
 
 Lemma valid_contract_execute_jump : Symbolic.ValidContractWithFuel 100 sep_contract_execute_jump fun_execute.
 Proof.
@@ -972,3 +976,11 @@ Proof.
      [right | left]; right;
      rewrite rightid_and_true; apply Hpc).
 Qed.
+
+
+(*
+    replace (bv.unsigned v3) with (bv.unsigned v3 + 0) by ring.
+    rewrite Z.add_comm with (n := 8).
+    apply Z.add_lt_mono; [assumption | reflexivity].
+    rewrite <-bv.of_Z_add, <-bv.of_N_add, bv.of_Z_unsigned, bv.of_N_bin, bv.add_comm;
+*)
